MPL/WPMonadExceptOf.lean
@@ -30,17 +30,16 @@ theorem MonadExcept.throwThe_apply [MonadExceptOf ε m] [WP m ps] :
 
 theorem Except.throw_apply :
   wp⟦MonadExceptOf.throw e : Except ε α⟧.apply Q = Q.2.1 e := by
-    simp only [wp, MonadExceptOf.throw, PredTrans.pushExcept_apply, PredTrans.throw, PredTrans.pure, Id.run, Except.error]
+    simp only [wp, PredTrans.pure, Id.run, MonadExceptOf.throw, PredTrans.pushExcept_apply]
 
 theorem ExceptT.throw_apply [Monad m] [WPMonad m ps] :
   wp⟦MonadExceptOf.throw e : ExceptT ε m α⟧.apply Q = Q.2.1 e := by
-    simp only [wp, throw, throwThe, MonadExceptOf.throw, ExceptT.mk, pure_pure, pure, PredTrans.pure,
-      PredTrans.pushExcept_apply, PredTrans.throw]
+    simp only [wp, MonadExceptOf.throw, ExceptT.mk, pure_pure, pure, PredTrans.pure,
+      PredTrans.pushExcept_apply]
 
 theorem EStateM.throw_apply :
   wp⟦MonadExceptOf.throw e : EStateM ε σ α⟧.apply Q = Q.2.1 e := by
-    simp only [wp, throw, throwThe, MonadExceptOf.throw, EStateM.throw, pure_pure, pure, PredTrans.pure,
-      PredTrans.pushArg_apply, PredTrans.throw]
+    simp only [wp, MonadExceptOf.throw, EStateM.throw]
 
 theorem ReaderT.throw_apply [WP m sh] [Monad m] [MonadExceptOf ε m] :
   wp⟦MonadExceptOf.throw (ε:=ε) e : ReaderT ρ m α⟧.apply Q = wp⟦MonadLift.monadLift (MonadExceptOf.throw (ε:=ε) e : m α) : ReaderT ρ m α⟧.apply Q := rfl
@@ -70,7 +69,7 @@ theorem Except.tryCatch_apply :
 theorem ExceptT.tryCatch_apply [Monad m] [WPMonad m ps] :
   wp⟦MonadExceptOf.tryCatch x h : ExceptT ε m α⟧.apply Q = wp⟦x⟧.apply (Q.1, fun e => wp⟦h e⟧.apply Q, Q.2.2) := by
     simp only [wp, MonadExceptOf.tryCatch, ExceptT.tryCatch, ExceptT.mk, bind_bind,
-      PredTrans.pushExcept_apply, PredTrans.bind_apply, PredTrans.tryCatch]
+      PredTrans.pushExcept_apply, PredTrans.bind_apply]
     congr
     ext x
     split <;> simp
@@ -80,7 +79,7 @@ theorem EStateM.tryCatch_apply {ε σ δ α x h Q} [EStateM.Backtrackable δ σ]
   wp⟦MonadExceptOf.tryCatch x h : EStateM ε σ α⟧.apply Q = fun s => wp⟦x⟧.apply (Q.1, fun e s' => wp⟦h e⟧.apply Q (restore s' (save s)), Q.2.2) s := by
     ext s;
     simp only [wp, MonadExceptOf.tryCatch, EStateM.tryCatch, bind_bind,
-      PredTrans.pushExcept_apply, PredTrans.bind_apply, PredTrans.tryCatch]
+      PredTrans.pushExcept_apply, PredTrans.bind_apply]
     cases x s <;> simp
 
 theorem ReaderT.tryCatch_apply [WP m sh] [Monad m] [MonadExceptOf ε m] :
